src/riscv/Platform/MetricMinimal.v
@@ -62,7 +62,7 @@ Section Riscv.
     getPrivMode := liftL0 id getPrivMode;
     setPrivMode := liftL1 id setPrivMode;
     step := liftL0 (addMetricInstructions 1) step;
-    raiseExceptionWithInfo{A} := liftL3 id (raiseExceptionWithInfo (A := A));
+    endCycle{A} := liftL0 id (@endCycle _ _ _ _ _ A);
   }.
 
   Arguments Memory.load_bytes: simpl never.
